

# Introductory Lectures on Optimization

## Homework (1)

Yang Yichou  
Student ID 3230105697

October, 2025

### Exercise 1. Norms

In this exercise, we will give some examples of norms and a useful theorem related to norms in finite dimensional vector space

1.  $l_p$  **norm**: The  $l_p$  norm is defined by

$$\|x\|_p = (\sum_{i=1}^n |x_i|^p)^{\frac{1}{p}} \quad (1)$$

where  $\mathbf{x} = (x_1, \dots, x_n) \in \mathbb{R}^n$  and  $p \geq 1$ .

- Please show that  $l_p$  norm is a norm.
- Please show that the following equality.

$$\lim_{p \rightarrow \infty} \|\mathbf{x}\|_p = \|\mathbf{x}\|_\infty = \max_{1 \leq i \leq n} |x_i|. \quad (2)$$

The  $l_\infty$  norm is defined as above

2. **Operator norms**: Suppose that  $\mathbf{A} \in \mathbb{R}^{m \times n}$ , which can be viewed as linear transformation from  $\mathbb{R}^n$  to  $\mathbb{R}^m$ . Please show that the following operator norms' equality.

- a. Let  $\|A\|_1 = \sup_{\mathbf{x} \in \mathbb{R}^n, \mathbf{x} \neq 0} \frac{\|\mathbf{Ax}\|_1}{\|\mathbf{x}\|_1}$ . Please show that

$$\|A\|_1 = \max_{1 \leq j \leq n} \sum_{i=1}^m |a_{ij}|. \quad (3)$$

- b. Let  $\|A\|_\infty = \sup_{\mathbf{x} \in \mathbb{R}^n, \mathbf{x} \neq 0} \frac{\|\mathbf{Ax}\|_\infty}{\|\mathbf{x}\|_\infty}$ . Please show that

$$\|A\|_\infty = \max_{1 \leq i \leq m} \sum_{j=1}^n |a_{ij}|. \quad (4)$$

**Proof of Exercise 1:** Write down your solutions step by step here.

1.a. A norm satisfies the following properties:

- positive definiteness:  $\|x\| \geq 0$ , and  $\|x\| = 0$  if and only if  $x = 0$
- linear:  $\forall a \in \mathbb{C}, \|ax\| = |a|\|x\|$
- triangle inequality:  $\|a\| + \|b\| \geq \|a + b\|$

Then we show that  $l_p$  satisfies all the properties listed above:

- (1)  $\|x\|_p = (\sum_{i=1}^n |x_i|^p)^{\frac{1}{p}} \geq 0$  is obvious

If  $\exists x_i \neq 0, i = 1, \dots, n$ . Then  $\|x\|_p = (\sum_{i=1}^n |x_i|^p)^{\frac{1}{p}} \geq |x_i| > 0$   
 $\therefore \|x\| = 0 \iff x = 0$ .

$$(2) \forall a \in \mathbb{C}, \|ax\|_p = (\sum_{i=1}^n |ax_i|^p)^{\frac{1}{p}} = (|a|^p)^{\frac{1}{p}} (\sum_{i=1}^n |x_i|^p)^{\frac{1}{p}} = |a| \|x\|_p$$

$$(3) \|a\|_p + \|b\|_p = (\sum_{i=1}^n |a_i|^p)^{\frac{1}{p}} + (\sum_{i=1}^n |b_i|^p)^{\frac{1}{p}}, \|a+b\|_p = (\sum_{i=1}^n |a_i+b_i|^p)^{\frac{1}{p}}$$

In coordinates,  $\forall i, |a_i|^p + |b_i|^p \geq |a_i+b_i|^p$

$$(\|a\|_p + \|b\|_p)^p \geq \sum_{i=1}^n |a_i|^p + \sum_{i=1}^n |b_i|^p \geq \sum_{i=1}^n |a_i+b_i|^p = (\|a+b\|_p)^p$$

$$\therefore \|a\|_p + \|b\|_p = \|a+b\|_p$$

1.b. Let  $M = \max_{1 \leq i \leq n} x_i, r$  be the number of different  $i, s.t. |x_i| = M$

$$\lim_{p \rightarrow \infty} \|x\|_p = \lim_{p \rightarrow \infty} (\sum_{i=1}^n |x_i|^p)^{\frac{1}{p}} = \lim_{p \rightarrow \infty} M \cdot (\sum_{i=1}^n (\frac{|x_i|}{M})^p)^{\frac{1}{p}} = M \cdot \lim_{p \rightarrow \infty} r^{\frac{1}{p}} = M = \|x\|_\infty$$

$$2.a. \mathbf{Ax} = \begin{bmatrix} a_{11} & \dots & a_{1n} \\ \dots & \dots & \dots \\ a_{m1} & \dots & a_{mn} \end{bmatrix} \begin{bmatrix} x_1 \\ \dots \\ x_n \end{bmatrix} = \begin{bmatrix} \sum_{i=1}^n a_{1i}x_i \\ \dots \\ \sum_{i=1}^n a_{mi}x_i \end{bmatrix}$$

$$\|A\|_1 = \sup_{x \in \mathbb{R}^n, x \neq 0} \frac{\|\mathbf{Ax}\|_1}{\|x\|_1} = \sup_{x \in \mathbb{R}^n, x \neq 0} \frac{\sum_{j=1}^m \sum_{i=1}^n |a_{ji}x_i|}{\sum_{i=1}^n |x_i|}$$

Let  $I$  be the only  $\arg \max_{1 \leq i \leq n} \sum_{j=1}^m |a_{ji}|$

$$\|A\|_1 = \max_{1 \leq i \leq n} \sum_{j=1}^m |a_{ji}| - \frac{\sum_{i \neq I} (\max_{1 \leq i \leq n} \sum_{j=1}^m |a_{ji}| - \sum_{j=1}^m |a_{ji}|) |x_i|}{\sum_{i=1}^n |x_i|} \geq \max_{1 \leq i \leq n} \sum_{j=1}^m |a_{ji}|$$

The equality holds when  $\forall i \neq I, x_i = 0$

$$\text{Then } \|A\|_1 = \max_{1 \leq j \leq n} \sum_{i=1}^m |a_{ij}|.$$

$$2.b. \|A\|_\infty = \sup_{x \in \mathbb{R}^n, x \neq 0} \frac{\|\mathbf{Ax}\|_\infty}{\|x\|_\infty} = \sup_{x \in \mathbb{R}^n, x \neq 0} \frac{\max_{1 \leq i \leq m} |\sum_{j=1}^n a_{ij}x_j|}{\max_{1 \leq i \leq n} |x_i|}$$

Recall the Holder inequation:  $p, q \in [1, +\infty), \frac{1}{p} + \frac{1}{q} = 1$ , we have  $\sum_{i=1}^n |a_i b_i| \leq (\sum_{i=1}^n |a_i|^p)^{\frac{1}{p}} (\sum_{i=1}^n |b_i|^q)^{\frac{1}{q}}$

$$\text{Let } p = 1, q = \infty, \sum_{i=1}^n |a_i b_i| \leq (\sum_{i=1}^n |a_i|) \max_{1 \leq i \leq n} |b_i|$$

$$\text{Then } \sum_{j=1}^n |a_{ij}x_j| \leq \sum_{j=1}^n |a_{ij}| \max_{1 \leq i \leq n} |x_i|$$

$$\therefore \frac{\|\mathbf{Ax}\|_\infty}{\|x\|_\infty} \leq \max_{1 \leq i \leq m} \sum_{j=1}^n |a_{ij}|$$

The equality holds when  $x_j = \overline{\text{sgn}(a_{ij})}$ , where  $\text{sgn}(z) = \begin{cases} \frac{z}{|z|}, & z \neq 0 \\ 0, & z = 0 \end{cases}$ , this ensures  $\max_{1 \leq i \leq n} |x_i| = 1$ .

$$\therefore \|A\|_\infty = \sup_{x \in \mathbb{R}^n, x \neq 0} \frac{\|\mathbf{Ax}\|_\infty}{\|x\|_\infty} = \max_{1 \leq i \leq m} \sum_{j=1}^n |a_{ij}|, x_j = \overline{\text{sgn}(a_{ij})}$$

□

## Exercise 2. Basis and Coordinates

Suppose that  $\{\mathbf{a}_1, \mathbf{a}_2, \dots, \mathbf{a}_n\}$  is a basis of an  $n$ -dimensional vector Space  $V$ .

1. Show that  $\{\lambda_1 \mathbf{a}_1, \lambda_2 \mathbf{a}_2, \dots, \lambda_n \mathbf{a}_n\}$  is also a basis of  $V$  for nonzero scalars  $\lambda_1, \lambda_2, \dots, \lambda_n$ .
2. Suppose that the coordinate of a vector  $\mathbf{v}$  under the basis  $\{\mathbf{a}_1, \dots, \mathbf{a}_n\}$  is  $\mathbf{x} = (x_1, x_2, \dots, x_n)$ 
  - a. What is the coordinate of  $\mathbf{v}$  under  $\{\lambda_1 \mathbf{a}_1, \dots, \lambda_n \mathbf{a}_n\}$ ?
  - b. What are the coordinates of  $\mathbf{w} = \sum_{i=1}^n \mathbf{a}_i$  under  $\{\mathbf{a}_1, \mathbf{a}_2, \dots, \mathbf{a}_n\}$  and  $\{\lambda_1 \mathbf{a}_1, \lambda_2 \mathbf{a}_2, \dots, \lambda_n \mathbf{a}_n\}$ ?  
Note that  $\lambda_i \neq 0 \forall i \in \{1, \dots, n\}$ .

**Proof of Exercise 2:** Write down your solutions step by step here.

1. To show  $\{\lambda_1 \mathbf{a}_1, \lambda_2 \mathbf{a}_2, \dots, \lambda_n \mathbf{a}_n\}$  is also a basis of  $V$ , we only need to show

(1)  $\forall i \neq j, i, j \in \{1, \dots, n\}, \langle \lambda_i \mathbf{a}_i, \lambda_j \mathbf{a}_j \rangle = 0$ ;

(2)  $\forall x \in V, x = \sum_{i=1}^n k_i \lambda_i \mathbf{a}_i$

Because  $\{\mathbf{a}_1, \mathbf{a}_2, \dots, \mathbf{a}_n\}$  is a basis of an  $n$ -dimensional vector Space  $V$ , we have

$\forall i \neq j, i, j \in \{1, \dots, n\}, \langle \mathbf{a}_i, \mathbf{a}_j \rangle = 0$

$\forall x \in V, x = \sum_{i=1}^n l_i \mathbf{a}_i$

(1)  $\forall i \neq j, \langle \lambda_i \mathbf{a}_i, \lambda_j \mathbf{a}_j \rangle = \lambda_i \overline{\lambda_j} \langle \mathbf{a}_i, \mathbf{a}_j \rangle = 0$

(2) Because  $\lambda_i \neq 0, \forall i$ , we can let  $k_i = \frac{l_i}{\lambda_i}$ , then  $\forall x \in V, x = \sum_{i=1}^n l_i \mathbf{a}_i = \sum_{i=1}^n k_i \lambda_i \mathbf{a}_i$

2.a. The coordinate of a vector  $\mathbf{v}$  under the basis  $\{\mathbf{a}_1, \dots, \mathbf{a}_n\}$  is  $\mathbf{x} = (x_1, x_2, \dots, x_n)$

$\iff \mathbf{v} = \sum_{i=1}^n x_i \mathbf{a}_i$

Then  $\mathbf{v} = \sum_{i=1}^n \frac{x_i}{\lambda_i} \lambda_i \mathbf{a}_i$

$\therefore$  the coordinate of  $\mathbf{v}$  under  $\{\lambda_1 \mathbf{a}_1, \dots, \lambda_n \mathbf{a}_n\}$  is  $\mathbf{x}' = (\frac{x_1}{\lambda_1}, \frac{x_2}{\lambda_2}, \dots, \frac{x_n}{\lambda_n})$

2.b.  $\mathbf{w} = \sum_{i=1}^n \mathbf{a}_i = \sum_{i=1}^n 1 \cdot \mathbf{a}_i \Rightarrow$  the coordinates of  $\mathbf{w} = \sum_{i=1}^n \mathbf{a}_i$  under  $\{\mathbf{a}_1, \mathbf{a}_2, \dots, \mathbf{a}_n\}$  is  $(1, 1, \dots, 1)$

Similarly,  $\mathbf{w} = \sum_{i=1}^n \mathbf{a}_i = \sum_{i=1}^n \frac{1}{\lambda_i} \cdot \lambda_i \mathbf{a}_i \Rightarrow$  the coordinates of  $\mathbf{w} = \sum_{i=1}^n \mathbf{a}_i$  under  $\{\lambda_1 \mathbf{a}_1, \lambda_2 \mathbf{a}_2, \dots, \lambda_n \mathbf{a}_n\}$  is  $(\frac{1}{\lambda_1}, \frac{1}{\lambda_2}, \dots, \frac{1}{\lambda_n})$

□

## Exercise 3. Differentiability

Let  $f : \mathbb{R}^n \rightarrow \mathbb{R}^m$  be a function,  $\mathbf{x}_0 \in \mathbb{R}^n$  be a point, and let  $L : \mathbb{R}^n \rightarrow \mathbb{R}^m$  be a linear transformation. We say that  $f$  is *differentiable* at  $\mathbf{x}_0$  with *derivative*  $L$  if we have

$$\lim_{\mathbf{x} \rightarrow \mathbf{x}_0; \mathbf{x} \neq \mathbf{x}_0} \frac{\|f(\mathbf{x}) - f(\mathbf{x}_0) - L(\mathbf{x} - \mathbf{x}_0)\|_2}{\|\mathbf{x} - \mathbf{x}_0\|_2} = 0 \quad (5)$$

We denote this derivative  $L$  by  $f'(\mathbf{x}_0)$ .

1. Let  $x, a \in \mathbb{R}^n$  and  $y \in \mathbb{R}^m$ . Consider the functions as follows. Please show that they are differentiable and find  $f'(\mathbf{x})$

(a)  $f(\mathbf{x}) = \mathbf{a}^T \mathbf{x}$ .

(b)  $f(\mathbf{x}) = \mathbf{x}^T \mathbf{x}$ .

(c)  $f(\mathbf{x}) = \|\mathbf{y} - \mathbf{A}\mathbf{x}\|_2^2$ , where  $\mathbf{A} \in \mathbb{R}^{m \times n}$ .

**Proof of Exercise 3:** Write down your solutions step by step here.

$$1.(a) f'(\mathbf{x}) = \left[ \frac{\partial f}{\partial x_1}, \frac{\partial f}{\partial x_2}, \dots, \frac{\partial f}{\partial x_n} \right] = [a_1, a_2, \dots, a_n] = \mathbf{a}^T$$

$$\lim_{\mathbf{x} \rightarrow \mathbf{x}_0; \mathbf{x} \neq \mathbf{x}_0} \frac{\|f(\mathbf{x}) - f(\mathbf{x}_0) - L(\mathbf{x} - \mathbf{x}_0)\|_2}{\|\mathbf{x} - \mathbf{x}_0\|_2} = \lim_{\mathbf{x} \rightarrow \mathbf{x}_0; \mathbf{x} \neq \mathbf{x}_0} \frac{\|\mathbf{a}^T \mathbf{x} - \mathbf{a}^T \mathbf{x}_0 - \mathbf{a}^T (\mathbf{x} - \mathbf{x}_0)\|_2}{\|\mathbf{x} - \mathbf{x}_0\|_2} = 0$$

$$(b) f'(\mathbf{x}) = \left[ \frac{\partial f}{\partial x_1}, \frac{\partial f}{\partial x_2}, \dots, \frac{\partial f}{\partial x_n} \right] = [2x_1, 2x_2, \dots, 2x_n] = 2\mathbf{x}^T$$

$$\lim_{\mathbf{x} \rightarrow \mathbf{x}_0; \mathbf{x} \neq \mathbf{x}_0} \frac{\|f(\mathbf{x}) - f(\mathbf{x}_0) - L(\mathbf{x} - \mathbf{x}_0)\|_2}{\|\mathbf{x} - \mathbf{x}_0\|_2} = \lim_{h \rightarrow 0} \frac{\|f(\mathbf{x}_0 + h) - f(\mathbf{x}_0) - 2\mathbf{x}_0^T h\|_2}{\|h\|_2} =$$

$$\lim_{h \rightarrow 0} \frac{\|\mathbf{x}_0^T \mathbf{x}_0 + 2\mathbf{x}_0^T h + h^T h - \mathbf{x}_0^T \mathbf{x}_0 - 2\mathbf{x}_0^T h\|_2}{\|h\|_2} = \lim_{h \rightarrow 0} \frac{\|h\|_2^2}{\|h\|_2} = 0$$

$$(c) \mathbf{x} = [x_1, \dots, x_n]^T, \mathbf{y} = [y_1, \dots, y_m]^T, \mathbf{A} = (a_{ij})_{m \times n}$$

$$f(\mathbf{x}) = \|\mathbf{y} - \mathbf{A}\mathbf{x}\|_2^2 = (\mathbf{y} - \mathbf{A}\mathbf{x})^T (\mathbf{y} - \mathbf{A}\mathbf{x}) = \mathbf{y}^T \mathbf{y} - 2\mathbf{y}^T \mathbf{A}\mathbf{x} + (\mathbf{A}\mathbf{x})^T \mathbf{A}\mathbf{x}$$

$$f(\mathbf{x})' = -2\mathbf{y}^T \mathbf{A} + 2(\mathbf{A}\mathbf{x})^T \mathbf{A} = 2(\mathbf{A}\mathbf{x} - \mathbf{y})^T \mathbf{A}$$

$$\lim_{\mathbf{x} \rightarrow \mathbf{x}_0; \mathbf{x} \neq \mathbf{x}_0} \frac{\|f(\mathbf{x}) - f(\mathbf{x}_0) - L(\mathbf{x} - \mathbf{x}_0)\|_2}{\|\mathbf{x} - \mathbf{x}_0\|_2} = \lim_{h \rightarrow 0} \frac{\|f(\mathbf{x}_0 + h) - f(\mathbf{x}_0) - L(h)\|_2}{\|h\|_2}$$

$$f(\mathbf{x}_0 + h) = \mathbf{y}^T \mathbf{y} - 2\mathbf{y}^T \mathbf{A}(\mathbf{x}_0 + h) + (\mathbf{x}_0 + h)^T \mathbf{A}^T \mathbf{A}(\mathbf{x}_0 + h) =$$

$$\mathbf{y}^T \mathbf{y} - 2\mathbf{y}^T \mathbf{A}\mathbf{x}_0 - 2\mathbf{y}^T \mathbf{A}h + \mathbf{x}_0^T \mathbf{A}^T \mathbf{A}\mathbf{x}_0 + 2\mathbf{x}_0^T \mathbf{A}^T \mathbf{A}h + h^T \mathbf{A}^T \mathbf{A}h$$

$$f(\mathbf{x}_0) = \mathbf{y}^T \mathbf{y} - 2\mathbf{y}^T \mathbf{A}\mathbf{x}_0 + \mathbf{x}_0^T \mathbf{A}^T \mathbf{A}\mathbf{x}_0$$

$$f(\mathbf{x}_0 + h) - f(\mathbf{x}_0) = -2\mathbf{y}^T \mathbf{A}h + 2\mathbf{x}_0^T \mathbf{A}^T \mathbf{A}h + h^T \mathbf{A}^T \mathbf{A}h = 2(\mathbf{A}\mathbf{x}_0 - \mathbf{y})^T \mathbf{A}h + h^T \mathbf{A}^T \mathbf{A}h$$

$$L(h) = 2(\mathbf{A}\mathbf{x}_0 - \mathbf{y})^T \mathbf{A}h$$

$$\therefore \lim_{\mathbf{x} \rightarrow \mathbf{x}_0; \mathbf{x} \neq \mathbf{x}_0} \frac{\|f(\mathbf{x}) - f(\mathbf{x}_0) - L(\mathbf{x} - \mathbf{x}_0)\|_2}{\|\mathbf{x} - \mathbf{x}_0\|_2} = \lim_{h \rightarrow 0} \frac{\|h^T \mathbf{A}^T \mathbf{A}h\|_2}{\|h\|_2} \leq \lim_{h \rightarrow 0} \frac{\|\mathbf{A}^T \mathbf{A}\|_2 \cdot \|h\|_2^2}{\|h\|_2} = 0$$

□

#### Exercise 4. Properties of Eigenvalues and Singular Values

1. Suppose the maximum eigenvalue, minimum eigenvalue of a given symmetric matrix  $A \in S^n$  are denoted by  $\lambda_{\max}(\mathbf{A})$  and  $\lambda_{\min}(\mathbf{A})$ , respectively. Please show that

$$\lambda_{\max}(\mathbf{A}) = \sup_{\mathbf{x} \in \mathbb{R}^n, \mathbf{x} \neq 0} \frac{\mathbf{x}^T \mathbf{A} \mathbf{x}}{\mathbf{x}^T \mathbf{x}}, \quad \lambda_{\min}(\mathbf{A}) = \inf_{\mathbf{x} \in \mathbb{R}^n, \mathbf{x} \neq 0} \frac{\mathbf{x}^T \mathbf{A} \mathbf{x}}{\mathbf{x}^T \mathbf{x}}. \quad (6)$$

(Hint: consider the orthogonal decomposition of  $\mathbf{A}$ .)

2. Suppose  $\mathbf{B} = (b_{ij}) \in \mathbb{R}^{m \times n}$  with maximum singular value  $\sigma_{\max}(\mathbf{B})$ .

- a. Let  $\|\mathbf{B}\|_2 := \sup_{\mathbf{x} \in \mathbb{R}^n, \mathbf{x} \neq 0} \frac{\|\mathbf{B}\mathbf{x}\|_2}{\|\mathbf{x}\|_2}$ . Please show that

$$\sigma_{\max}(\mathbf{B}) = \|\mathbf{B}\|_2. \quad (7)$$

- b. Please show that

$$\sigma_{\max}(\mathbf{B}) = \sup_{\mathbf{x} \in \mathbb{R}^m, \mathbf{y} \in \mathbb{R}^n, \mathbf{x}, \mathbf{y} \neq 0} \frac{\mathbf{x}^T \mathbf{B} \mathbf{y}}{\|\mathbf{x}\|_2 \|\mathbf{y}\|_2} \quad (8)$$

3. Please show the following two equalities:

$$f(\mathbf{y}) - f(\mathbf{x}) = \int_0^1 \nabla f(\mathbf{x} + t(\mathbf{y} - \mathbf{x}))^T (\mathbf{y} - \mathbf{x}) dt \quad (9)$$

$$\nabla f(\mathbf{y}) - \nabla f(\mathbf{x}) = \int_0^1 \nabla^2 f(\mathbf{x} + t(\mathbf{y} - \mathbf{x})) (\mathbf{y} - \mathbf{x}) dt \quad (10)$$

(Hint: you may consider the function  $g(t) = f(\mathbf{x} + t(\mathbf{y} - \mathbf{x}))$  and apply the fundamental theorem of calculus.)

4. Suppose that  $f : \mathbb{R}^n \rightarrow \mathbb{R}$  is twice continuously differentiable, and the gradient of  $f$  is Lipschitz continuous, i.e.,

$$\|\nabla f(\mathbf{x}) - \nabla f(\mathbf{y})\|_2 \leq L\|\mathbf{x} - \mathbf{y}\|_2, \forall \mathbf{x}, \mathbf{y} \in \mathbb{R}^n, \quad (11)$$

where  $L \geq 0$  is Lipschitz constant. Please show that  $\lambda_{\max}(\nabla^2 f(\mathbf{x})) \leq L$  for any  $\mathbf{x} \in \mathbb{R}^n$ , where  $\lambda_{\max}(\nabla^2 f(\mathbf{x}))$  is the largest eigenvalue of  $\nabla^2 f(\mathbf{x})$ .

**Proof of Exercise 4:** Write down your solutions step by step here.

1. Because  $\mathbf{A}$  is symmetric matrix,  $\mathbf{A}$  can be decomposed to  $\mathbf{A} = \mathbf{Q}\mathbf{\Lambda}\mathbf{Q}^T$ , where  $\mathbf{Q}$  is an orthogonal matrix,  $\mathbf{Q}^T\mathbf{Q} = \mathbf{Q}\mathbf{Q}^T = \mathbf{I}$ ,  $\mathbf{\Lambda} = \text{diag}\{\lambda_1, \dots, \lambda_n\}$ , assume  $\lambda_1 \geq \dots \geq \lambda_n$ .

Then let  $\mathbf{x} = \mathbf{Q}\mathbf{y}$ , we have

$$\frac{\mathbf{x}^T \mathbf{A} \mathbf{x}}{\mathbf{x}^T \mathbf{x}} = \frac{\mathbf{y}^T \mathbf{Q}^T \mathbf{Q} \mathbf{\Lambda} \mathbf{Q}^T \mathbf{Q} \mathbf{y}}{\mathbf{y}^T \mathbf{Q}^T \mathbf{Q} \mathbf{y}} = \frac{\mathbf{y}^T \mathbf{\Lambda} \mathbf{y}}{\mathbf{y}^T \mathbf{y}} = \frac{\sum_{i=1}^n \lambda_i y_i^2}{\sum_{i=1}^n y_i^2}$$

Select  $\mathbf{x}$  that makes  $\mathbf{y} = (1, 0, \dots, 0)^T$ , we have  $\sup_{\mathbf{x} \in \mathbb{R}^n, \mathbf{x} \neq 0} \frac{\mathbf{x}^T \mathbf{A} \mathbf{x}}{\mathbf{x}^T \mathbf{x}} = \lambda_1 = \lambda_{\max}(\mathbf{A})$ .

Similarly, select  $\mathbf{x}$  that makes  $\mathbf{y} = (0, \dots, 0, 1)^T$ , we have  $\inf_{\mathbf{x} \in \mathbb{R}^n, \mathbf{x} \neq 0} \frac{\mathbf{x}^T \mathbf{A} \mathbf{x}}{\mathbf{x}^T \mathbf{x}} = \lambda_n = \lambda_{\min}(\mathbf{A})$ .

2.a. w.l.o.g. Assume  $n \leq m$

Matrix  $\mathbf{B}$  has an SVD:  $\mathbf{B} = \mathbf{U}\mathbf{\Sigma}\mathbf{V}^T$ , where  $\mathbf{U}, \mathbf{V}$  are both orthogonal matrix,  $\mathbf{U}^T\mathbf{U} = \mathbf{V}^T\mathbf{V} = \mathbf{I}$ ,  $\mathbf{\Sigma} = \text{diag}\{\sigma_1, \dots, \sigma_n\}$ , assume  $\sigma_1 \geq \dots \geq \sigma_n$ .

Then let  $\mathbf{x} = \mathbf{V}\mathbf{y}$ , we have

$$\|\mathbf{B}\|_2^2 = \frac{\|\mathbf{B}\mathbf{x}\|_2^2}{\|\mathbf{x}\|_2^2} = \frac{\|\mathbf{U}\mathbf{\Sigma}\mathbf{V}^T\mathbf{V}\mathbf{y}\|_2^2}{\|\mathbf{V}\mathbf{y}\|_2^2} = \frac{\|\mathbf{U}\mathbf{\Sigma}\mathbf{y}\|_2^2}{\|\mathbf{V}\mathbf{y}\|_2^2} = \frac{\|\mathbf{\Sigma}\mathbf{y}\|_2^2}{\|\mathbf{y}\|_2^2} = \frac{\sum_{i=1}^n \sigma_i^2 y_i^2}{\sum_{i=1}^n y_i^2}$$

Select  $\mathbf{x}$  that makes  $\mathbf{y} = (1, 0, \dots, 0)^T$ , we have  $\|\mathbf{B}\|_2^2 = \sigma_{\max}^2(\mathbf{B})$

$\therefore \|\mathbf{B}\|_2 = \sigma_{\max}(\mathbf{B})$

2.b. let  $\mathbf{x} = \mathbf{U}\mathbf{a}, \mathbf{y} = \mathbf{V}\mathbf{b}$ , we have

$$\frac{\mathbf{x}^T \mathbf{B} \mathbf{y}}{\|\mathbf{x}\|_2 \|\mathbf{y}\|_2} = \frac{\mathbf{a}^T \mathbf{U}^T \mathbf{U} \mathbf{\Sigma} \mathbf{V}^T \mathbf{V} \mathbf{b}}{\|\mathbf{U}\mathbf{a}\|_2 \|\mathbf{V}\mathbf{b}\|_2} = \frac{\mathbf{a}^T \mathbf{\Sigma} \mathbf{b}}{\|\mathbf{a}\|_2 \|\mathbf{b}\|_2} = \frac{\sum_{i=1}^n \sigma_i a_i b_i}{\|\mathbf{a}\|_2 \|\mathbf{b}\|_2}$$

Recall the Cauchy-Schwarz inequation:

$$|\sum_{i=1}^n \sigma_i a_i b_i| \leq \sqrt{\sum_{i=1}^n \sigma_i^2 a_i^2} \sqrt{\sum_{i=1}^n b_i^2} \leq \sigma_1 \|\mathbf{a}\|_2 \|\mathbf{b}\|_2$$

$$\therefore \sup_{\mathbf{x} \in \mathbb{R}^m, \mathbf{y} \in \mathbb{R}^n, \mathbf{x}, \mathbf{y} \neq 0} \frac{\mathbf{x}^T \mathbf{B} \mathbf{y}}{\|\mathbf{x}\|_2 \|\mathbf{y}\|_2} = \sigma_1 = \sigma_{\max}(\mathbf{B})$$

3. The fundamental theorem of calculus is:

$$\int_a^b f(x) dx = F(b) - F(a), F(x)' = f(x)$$

Let  $g(t) = f(\mathbf{x} + t(\mathbf{y} - \mathbf{x}))$ ,  $g(0) = f(\mathbf{x})$ ,  $g(1) = f(\mathbf{y})$

$\nabla g(t) = \nabla f(\mathbf{x} + t(\mathbf{y} - \mathbf{x}))^T (\mathbf{y} - \mathbf{x})$

Then apply the fundamental theorem of calculus:

$$g(1) - g(0) = f(\mathbf{y}) - f(\mathbf{x}) = \int_0^1 \nabla g(t) dt = \int_0^1 \nabla f(\mathbf{x} + t(\mathbf{y} - \mathbf{x}))^T (\mathbf{y} - \mathbf{x}) dt$$

For  $\nabla g(t) = \nabla f(\mathbf{x} + t(\mathbf{y} - \mathbf{x}))^T (\mathbf{y} - \mathbf{x})$ , we have  
 $\nabla g(1) = \nabla f(\mathbf{x})^T (\mathbf{y} - \mathbf{x})$ ,  $\nabla g(0) = \nabla f(\mathbf{y})^T (\mathbf{y} - \mathbf{x})$   
 Then apply the fundamental theorem of calculus:

$$\nabla g(1) - \nabla g(0) = (\nabla f(\mathbf{y}) - \nabla f(\mathbf{x}))^T (\mathbf{y} - \mathbf{x}) = \int_0^1 \nabla^2 g(t) dt = \int_0^1 \nabla^2 f(\mathbf{x} + t(\mathbf{y} - \mathbf{x}))^T (\mathbf{y} - \mathbf{x})^2 dt$$

Thus, we have

$$\nabla f(\mathbf{y}) - \nabla f(\mathbf{x}) = \int_0^1 \nabla^2 f(\mathbf{x} + t(\mathbf{y} - \mathbf{x})) (\mathbf{y} - \mathbf{x}) dt$$

4. To show  $\lambda_{max}(\nabla^2 f(\mathbf{x})) \leq L$ , according to (6), we only need to show  $\sup_{\|\mathbf{v}\|=1} \mathbf{v}^T \nabla^2 \mathbf{f}(\mathbf{x}) \mathbf{v} \leq L$

Similar to the solution to question number 3, let  $g(t) = f(\mathbf{x} + t\mathbf{v})$

Then  $\nabla g(t) = \nabla f(\mathbf{x} + t\mathbf{v})^T \mathbf{v}$ ,  $\nabla^2 g(t) = \mathbf{v}^T \nabla^2 f(\mathbf{x} + t\mathbf{v}) \mathbf{v}$

$f$  is twice continuously differentiable, so we have: (remember that  $\mathbf{v}$  is a unit vector)

$$\forall t, \|\nabla f(\mathbf{x} + t\mathbf{v}) - \nabla f(\mathbf{x})\|_2 \leq Lt$$

On the direction of  $\mathbf{v}$ , we have:

$$|\nabla f(\mathbf{x} + t\mathbf{v})^T \mathbf{v} - \nabla f(\mathbf{x})^T \mathbf{v}| \leq Lt$$

$$|\nabla g(t) - \nabla g(0)| \leq Lt$$

Applying the Lagrange's Mean Value Theorem:

$$\exists \xi \in (0, t), |\nabla^2 g(\xi)| = \frac{|\nabla g(t) - \nabla g(0)|}{t} \leq L$$

$$\therefore \forall \mathbf{v}, \mathbf{v}^T \nabla^2 f(\mathbf{x} + t\mathbf{v}) \mathbf{v} \leq L$$

Let  $t \rightarrow 0$ ,  $\lambda_{max}(\nabla^2 f(\mathbf{x})) = \sup_{\|\mathbf{v}\|=1} \mathbf{v}^T \nabla^2 \mathbf{f}(\mathbf{x}) \mathbf{v} \leq L$

□